Write call single-step, single-thread unwind
This commit finishes a proof of the single-step, single-threaded
unwinding condition for just the write call and just in the case where
the label of the node making the call does flow to the label of the
observer. Several new smaller theorems are introduced but admitted for
now. They should be relatively simple. The files are reorganized a bit.

experimental/ni_coq/vfiles/LowEquivalences.v
@@ -26,6 +26,8 @@ Inductive chan_low_eq: level -> channel -> channel -> Prop :=
     | ChNoFlow ell ch1 ch2
         (* if the level is not high enough to read either channel,
         * they both look the same to observers at this level *)
+        (Hlbl_eq: ch1.(clbl) = ch2.(clbl))  
+                (* Hlbl_eq makes the labels of channels publicly observable *)
         (H1: ~(ch1.(clbl) <<L ell))
         (H2: ~(ch2.(clbl) <<L ell)):
         chan_low_eq ell ch1 ch2.
@@ -33,12 +35,12 @@ Inductive chan_low_eq: level -> channel -> channel -> Prop :=
 Inductive node_low_eq: level -> node -> node -> Prop :=
     | NodeEq ell n1 n2 (H: n1 = n2): node_low_eq ell n1 n2
     | NodeNoFlow ell n1 n2
+        (Hlbl_eq: n1.(nlbl) = n2.(nlbl))
+                (* Hlbl_eq makes the labels of nodes publicly observable *)
         (H1: ~(n1.(nlbl) <<L ell))
         (H2: ~(n2.(nlbl) <<L ell)):
         node_low_eq ell n1 n2.
 
-(* Is there may a better way to write these using the finset / finmap
-* libs *)
 Definition chan_state_low_eq (ell: level)(chs1 chs2: chan_state): Prop :=
     forall h, (match (chs1 .[?h]), (chs2 .[?h]) with
         | None, None => True
