experimental/ni_coq/vfiles/Unwind.v
@@ -1,0 +1,105 @@
+Require Import Coq.Lists.List.
+Import ListNotations.
+From OakIFC Require Import
+    Parameters
+    RuntimeModel
+    EvAugSemantics
+    Events
+    LowEquivalences
+    Lattice
+    NIUtilTheorems.
+From mathcomp Require Import all_ssreflect finmap.
+From RecordUpdate Require Import RecordSet.
+Import RecordSetNotations.
+
+(*============================================================================
+ Unwinding Theorems
+============================================================================*)
+(*
+This file contains theorems that prove "the unwinding condition" for 
+various single pure functions. An unwinding condition is a single step of
+noninterference.
+*)
+
+(*
+It might be better to write them using something like this in the future:
+
+Definition state_unwind (f: state -> state):
+    forall ell s1 s2, 
+        state_low_eq ell s1 s2 ->
+        state_low_eq ell (f s1) (fs 2)
+
+but we have to fix the way the definitions are curried.
+*)
+
+Theorem chan_append_unwind:
+    forall ell ch1 ch2 msg,
+    chan_low_eq ell ch1 ch2 ->
+    chan_low_eq ell (chan_append ch1 msg) (chan_append ch2 msg).
+Proof.
+Admitted. (* WIP // TODO *)
+
+Theorem state_upd_unwind_from_leqn:
+    forall ell id n1 n2 s1 s2,
+    node_low_eq ell n1 n2 ->
+    state_low_eq ell s1 s2 ->
+    state_low_eq ell (state_upd_node id n1 s1) (state_upd_node id n2 s2).
+Proof.
+    intros. inversion H0. 
+    split.
+    - (* nodes *) 
+        intros id'. destruct (id' =P id). 
+        + (* eq *) 
+            rewrite e;
+            rewrite !state_upd_node_eq; assumption.
+        + (* neq *) 
+            rewrite !state_upd_node_neq.
+            apply (H1 id');  assumption.
+    - (* chans *)
+        assumption. assumption. apply H2.
+Qed.
+
+Theorem set_call_unwind: forall ell id c s1 s2,
+    state_low_eq ell s1 s2 ->
+    state_low_eq ell (s_set_call s1 id c) (s_set_call s2 id c).
+Proof.
+    intros. inversion H; subst.
+    unfold s_set_call.
+    destruct (s1.(nodes).[? id]) eqn:E1; destruct (s2.(nodes).[? id]) eqn:E2.
+    - (* some, some *)
+        assert (E: node_low_eq ell 
+            (n <| ncall ::= (fun=> c) |>)
+            (n0 <| ncall ::= (fun=> c) |>)).
+        {
+            specialize (H0 id). rewrite E1 E2 in H0.
+            inversion H0; subst.
+            constructor; reflexivity.
+            constructor 2; assumption.
+        }
+        eapply state_upd_unwind_from_leqn; assumption.
+    - (* some, none *)
+        exfalso. specialize (H0 id).
+        rewrite E1 E2 in H0.
+        assumption.
+    - (* none, some *)
+        exfalso. specialize (H0 id).
+        rewrite E1 E2 in H0.
+        assumption.
+    - split; assumption.
+Qed.
+
+Theorem call_havoc_unwind: forall ell id c t1 t2 t1' t2',
+    (trace_low_eq ell t1 t2) ->
+    (t1' = head_set_call t1 id c) ->
+    (t2' = head_set_call t2 id c) ->
+    (trace_low_eq ell t1' t2').
+Proof.
+    intros.
+    destruct t1, t2; simpl in *; subst.
+    - (* nil, nil *) constructor.
+    - (* nil, not nil *) inversion H.
+    - (* not nil, nil *) inversion H.
+    - destruct p. destruct p0. inversion H; subst.
+    constructor 2; try assumption.
+    eapply set_call_unwind; assumption.
+Qed.
